[Typeclass Refinement] wp_simp tactic added

theories/refinement.v
@@ -9,11 +9,9 @@ Definition Par' {A1 A2 A3} (e: free A1) (e': free A2) (k: A1 * A2 -> free A3) :=
 Definition refinement {A: Type} (m m': free A): Prop :=
   forall (φ: A -> Prop), safe m' φ -> safe m φ.
 
-Class Refinement {A} (e e': free A) := { refine_expr : refinement e' e }.
-Set Typeclasses Depth 10.
-Set Typeclasses Strict Resolution.
-Set Typeclasses Debug.
+Class Refinement {A} (e' e: free A) := { refine_expr : refinement e' e }.
 
+Global Hint Mode Refinement - ! - : typeclass_instances.
 
 
 (** TODO: define a nice notation *)
@@ -28,9 +26,9 @@ Instance safe_refinement_par {A1 A2 A}
   (φ : A1 * A2 → Prop)
   (k : A1 * A2 → free A)
   (ko: () -> free A)
-  (R1: Refinement m1 m1')
-  (R2: Refinement m2 m2'):
-  Refinement (par m1 m2) (par m1' m2').
+  (R1: Refinement m1' m1)
+  (R2: Refinement m2' m2):
+  Refinement (par m1' m2') (par m1 m2).
 Proof.
   constructor.
   intros φ' (φ1 & φ2 & Hm1' & Hm2 & H)%invert_safe_par.
@@ -46,18 +44,20 @@ Qed.
 Instance refinement_sym A: Reflexive (@refinement A).
 Proof. now intros???. Qed.
 
-Lemma safe_refinement_refl {A}
-  (m: free A) : Refinement m m.
+#[global]
+Instance safe_refinement_refl {A}
+  (m: free A) : Refinement m m | 999.
 Proof. constructor. reflexivity. Qed.
 
 #[global]
 Instance refinement_trans A: Transitive (@refinement A).
-Proof. intros???????; auto. Qed.
+   Proof. intros???????; auto. Qed.
 
-#[global]
+   (* #[global]
 Instance safe_refinement_trans {A}
-(m m' m'': free A) (R1: Refinement m m') (R2: Refinement m' m''): Refinement m m''.
-Proof. constructor. transitivity m'; apply refine_expr. Qed.
+  (m m' m'': free A)
+  (R1: Refinement m m') (R2: Refinement m' m''): Refinement m m''.
+      Proof. constructor. transitivity m'; apply refine_expr. Qed. *)
 
 #[global]
 Instance refinement_proper_par A B:
@@ -82,17 +82,19 @@ Proof.
 Qed.
 
 #[global]
-Instance safe_refinement_Par A B C (ko: A * B -> free C) (a a': free A) (b b': free B)
-  (R1: Refinement a a')
-  (R2: Refinement b b'):
-  Refinement (Par a b ko next) (Par a' b' ko next).
+Instance safe_refinement_Par A B C
+  (ko: A * B -> free C) (a a': free A) (b b': free B)
+  (R1: Refinement a' a)
+  (R2: Refinement b' b):
+  Refinement (Par a' b' ko next) (Par a b ko next).
 Proof.
   constructor.
   intros φ (φ1&φ2&Ha&Hb&H)%invert_safe_par.
   rewrite safe_par.
   exists φ1, φ2.
-  repeat split; eauto;
-  now apply refine_expr.
+  repeat split; eauto.
+  - now apply R1.(refine_expr).
+  - now apply R2.(refine_expr).
 Qed.
 
 #[global]
@@ -106,9 +108,18 @@ Qed.
 #[global]
 Instance safe_refinement_call_ret_ret A B C
   (a: A) (b: B) (k: A * B -> free C):
-  Refinement (k (a, b)) (Par (Ret a) (Ret b) k next).
+  Refinement (Par (Ret a) (Ret b) k next) (k (a, b)).
 Proof.
   constructor.
   intros φ H.
   now apply prove_safe_par_ret_ret.
+Qed.
+
+Lemma refinement_simpl {A} (e e': free A) φ:
+  Refinement e' e
+  -> safe e φ
+  -> safe e' φ.
+Proof.
+  intros R H.
+  now apply R.(refine_expr).
 Qed.
